# Algebraic data types

Kinds -> Types -> Values

Types are static and resolve at compile time whereas values are dynamic and resolve at runtime.

```haskell
data Doggies a = 
    Husky a
  | Mastiff a
  deriving (Eq, Show)
```

1. Doggies is a type construcotr
2. Doggies has kind '* -> *'
3. Doggies String has kind *
4. Husky 10 has type Num a => Doggies a
5. Husky (10 :: Integer) has type Doggies Integer
6. Mastiff "Scooby Doo" has type Doggies [Char]
7. It's both a type constructor and a data constructor
8. It doesn't make sense to ask for the type of DogueDeBordeaux given that it isn't a value level constant.
9. DogueDeBordeaux "doggie!" has type DogueDeBordeaux [Char]

### newtype

The newtype is a data type that can only ever have a single unary data constructor.

```haskell
newtype Goats = Goats Int deriving (Eq, Show)
```
At runtime Goats is really an Int since the representation of newtypes and the type it contains are the same. 

newtypes can help give context to our types.

cf. 
tooManyGoats :: Int -> Bool
tooManyGoats' :: Goats -> Bool


### Language pragmas

These are extensions or special instructions telling the compiler to process input in ways beyond what the standard provides for.

The "GeneralizedNewtypeDeriving" language pragma tells the compiler to allow our newtype to reply on same typeclass instances of the type it contains. 

```haskell
{-# LANGUAGE GeneralizedNewtypeDeriving #-}

class TooMany a where
  tooMany :: a -> Bool

instance TooMany Int where
  tooMany n = n > 42

newtype Goats = 
  Goats Int deriving (Eq, Show, TooMany)

-- Goats has the same typeclass instances as the type it contains; namely, the typeclass instances that Int has
```

Intermission exercise
Question 3 (p.397)

### Record syntax 

Record syntax is a way to write data constructors with labelled type arguments that let you reference the type arguments and which also serve as projection functions for acccessing them.

```haskell
data Person = Person { name :: String, age :: Int } deriving (Eq, Show)

name :: Person -> String
name (Person n _) = n

age :: Person -> Int
age (Person _ a) = a

x = Person "jared" 22
age x --returns 22
name x --returns "jared"
```

### Normal form (How does this work?)

Writing product data types in normal involves writing their data constructors as a 'sum of products'

Product types distribute over sum types

```haskell
 a * (b + c) -> (a * b) + (a * c)
--  assume a, b and c are set cardinalities
```
A stricter interpretation of normal form involves representing products with tuples and sums with Either.


While we can partially apply data constructors just like with partial function applications, with record syntax we must provide all type arguments. If some field or type argument is not initialised, then we run into bottom or undefined and when we do so we run into an infinite computation. 


Best practices with product types using record syntax

It's best to extract out product types defined using record syntax into their own data definitions and then reference their type constructors in any data types that make use of them.


The cardinality of a function a -> b is $b^a$

Intermission exercises p.423
1. Quad is a sum type with cardinality 4
2. A sum type of two Quad types has a cardinality of 8
3. prodQuad :: (Quad, Quad) has cardinality 16
4. funcQuad :: Quad -> Quad has cardinality 4 ^ 4 = 256
5. prodTBool :: (Bool, Bool, Bool) has cardinality 2 * 2 * 2 = 8
6. gTwo :: Bool -> Bool -> Bool has cardinality 4 ^ 2 = (4 ^ 1) * 4 = 4 * 4 = 16
7. fTwo :: Bool -> Quad -> Quad has cardinality 256 ^ 2 = 65536

We can think of kinds as generalising or quantifying over types and types as generalising or quantifying over terms.

The hierarchy looks something like this:
Kinds
Types (includes type constants, variables and functions)
Terms (includes value constants, variables and functions)

A function at the term level

not :: Bool -> Bool

A function at the type level

List :: * -> *


#### Mapping binary trees (p.430)

mapTree function for mapping binary trees

With a map, the structure of our tree won't change but the values inhabiting each node will
Traverse through the binary tree by looking at left, right then the node itself and applying a function each time

```haskell
mapTree :: (a -> b) -> BinaryTree a -> BinaryTree b 
```

If we find a Leaf, we return itself
But if we stumble on a Node, then we make a recursive call 

```haskell
mapTree f (Node Leaf 0 Leaf) = Node Leaf (f 0) Leaf
mapTree f (Node Leaf 2 (Node Leaf 3 Leaf)) = Node Leaf (f 2) (Node Leaf 3 Leaf)
                                           = Node Leaf (f 2) (mapTree f (Node Leaf 3 Leaf))
                                           = Node Leaf (f 2) (Node Leaf (f 3) Leaf)
```

What about a binary tree that branches both left and right? 
How do we know whether to traverse the left or right subtree first?
We specify that we always look at the current node first, then the left node and finally the right node. 
  
Consider: 
```haskell
Node (Node Leaf 1 leaf) 0 (Node Leaf 2 Leaf) 

mapTree f (Node (Node Leaf 1 Leaf) 0 (Node Leaf 2 Leaf)) = ???
```

First, we check the left node, if its not a leaf, we map the left subtree whilst keeping the rest of the tree unchanged.
Then we check the right node, if its not a leaf, we map the right subtree whilst keeping the rest of the tree unchanged.
Finally we map the value at the top most node with the rest of the tree intact.

The idea is something along these lines:
```haskell
mapTree :: (a -> b) -> BinaryTree a -> BinaryTree b 
mapTree f Leaf = Leaf
mapTree f (Node left a right)
    | left == Node && right == Node = Node (mapTree f left) (f a) (mapTree f right)
    | left == Node                  = Node (mapTree f left) (f a) right
    | right == Node                 = Node left (f a) (mapTree f right)
    | otherwise                     = Node left (f a) right
```

But we can't check whether 'left' or 'right' is a Node or Leaf by using (==). 

Why not just always make recursive calls for both the left and right subtrees until we reach a Leaf?

Final solution:
```haskell
mapTree :: (a -> b) -> BinaryTree a -> BinaryTree b 
mapTree f Leaf = Leaf
mapTree f (Node left a right) = Node (mapTree f left) (f a) (mapTree f right)
```


#### Creating a list from a binary tree

With preorder the order is: current -> left -> right
With inorder, the order is: left -> current -> right
With postorder, the order is: left -> right -> current

```haskell
preorder :: BinaryTree a -> [a]
preorder Leaf = []
preorder (Node left a right) = [a] ++ preorder left ++ preorder right

inorder :: BinaryTree a -> [a]
inorder Leaf = []
inorder (Node left a right) = inorder left ++ [a] ++ inorder right 

postorder :: BinaryTree a -> [a]
postorder Leaf = []
postorder (Node left a right) = postorder left ++ postorder right ++ [a]
```

#### Foldr for binary tress

We have to specify an order in which to fold over our tree.

```haskell
data BinaryTree a = 
    Leaf
  | Node (BinaryTree a) a (BinaryTree a)
  deriving (Eq, Ord, Show)

-- let's first try an inorder traversal
foldTree :: (a -> b -> b) -> b -> BinaryTree a -> b
foldTree f acc Leaf = acc
foldTree f acc (Node left a right) = f a (foldTree f acc left)


foldTree f acc Leaf = acc
foldTree f acc (Node left a right) 
  | foldTree f acc left == acc && foldTree f acc right == acc = f a acc
  | foldTree f acc left == acc                                = f a (foldTree f acc right)
  | foldTree f acc right == acc                               = f a (foldTree f acc left)
  | otherwise                                                 = f a (foldTree f (foldTree f acc right) left)
```

```haskell
-- preorder
foldTree f acc Leaf = acc
foldTree f acc (Node left a right) = f a (foldTree f (foldTree f acc right) left)

-- postorder
foldTree f acc Leaf = acc
foldTree f acc (Node left a right) = foldTree f (foldTree f (f a acc) right) left

-- inorder
foldTree f acc Leaf = acc
foldTree f acc (Node left a right) = foldTree f (f a (foldTree f acc right)) left
```

With preorder traversal, we first fold over the right subtree, then the left subtree and finally the current node.
With postorder traversal, we first fold over the current node, then the right subtree and finally the left subtree.
With inorder traversal, we first fold over the right subtree, then over the current node and finally over the left subtree.

With inorder traversal, the accumulator to our left subtree is the accumulated value after folding over the right subtree and the current node. 
Mutatis mutandis for preorder and postorder traversals.



#### Defining a map function for binary trees in terms of the foldr function for binary trees

```haskell
mapTree' :: (a -> b) -> BinaryTree a -> BinaryTree b
mapTree' f tree = 

```

unfinished



### The VigenÃ¨re cipher

Step1
Select a word to encode your message with

Step2
Pad your word by cycling through its letters until its length matches the message to be encoded.

Step3
Then shift the position of each letter of the message to be encoded by the alphabetical rank of the corresponding letter in the word doing the encoding.


Step2 is the same as mapping each letter of our message to the result of applying `mod` to its index and the length of the encoding word.

Then we map each index to the letter in the encoding word.

Then we map the resulting list to its position in the alphabet. This will determine by how many positions we need to right shift. We can do this by first converting each letter to its character code and then subtract 97 to ensure that 'a' corresponds to 0 positions, 'b' with 1 position and so on and so forth.


e.g. 
word = "dog"
msg = "jared"
"jared"
"dogdo"

"01234"
"01201"

"jared" -> [0, 1, 2, 0, 1] 
        -> map (\x -> "dog" !! x) [0, 1, 2, 0, 1]
        -> "dogdo"
        -> map (\x -> ord x - 97) "dogdo"

call the result list 'encoding'

shiftedWord = zipWith (\letter numOfPlaces -> ord letter + numOfPlaces) msg encoding

Then we need to convert unicode back to letters.
['a'..'z']
map (flip mod 26 . ord) ['a'..'z']

shiftedWord -> map (flip mod 26) shiftedWord
	    -> 

```haskell
encodingWord :: String
encodingWord = "dog"

encode :: String -> [Int]
encode = map (flip . mod $ length encodingWord)

-- Map indexes to letters of our encodingWord
-- [0, 1, 2, 0, 1] -> ['d', 'o', 'g', 'd', 'o']
encode2 :: [Int] -> [Char]
encode2 = map (\x -> encodingWord !! x)

-- Map letters of our encodingWord to the number of right shifts that they represent
-- "dogdo" -> [3, 14, 6, 3, 14]
encode3 :: [Char] -> [Int]
encode3 = map (flip (-) 97 . ord)


-- To go from unicode to letters, we can look through the alphabet and the letter s.t. (flip mod 26 . ord) letter == 'our unicode' is true, will  be the corresponding letter.

-- Returns the letter of the alphabet that matches our argument
equalsX :: Char -> Char
equalsX x = filter ((==x) . flip mod 26 . ord) ['a'..'z']

-- Takes an encoding word and a message to encode and returns the result of encoding the message with the encoding word using a vigenere cipher
encodeMsg :: String -> String -> String
encodeMsg encodingWord msg = zipWith (\shiftCount letter -> equalsX $ ord letter + shiftCount) encodingWord msg
```


### As-patterns

They have the form `var@pattern`

assigns matched pattern after "@" symbol to the symbol preceding "@" so that the preceding symbol can be used in the RHS expression.

e.g.
```haskell
f :: Show a => (a, b) -> IO (a, b)
f t@(a, _) = do
  print a
  return t
```