# Traversable

```haskell
class (Functor t, Foldable t) => Traversable t where
  traverse :: Applicative f => (a -> f b) -> t a -> f (t b)
  sequenceA :: Applicative f => t (f a) -> f (t a)
  mapM :: Monad m => (a -> m b) -> t a -> m (t b)
  sequence :: Monad m => t (m a) -> m (t a)
```

fmap :: Functor f => (a -> b) -> f a -> f b

`sequenceA` turns a structure inside out.
Note that `traverse` is just `(sequenceA . ) . fmap`. In some sense, `traverse` is a special `fmap` that keeps the Applicative structure on the outside.

Similarly, for the bind function defined for Monads,
```haskell
(=<<) :: Monad m => (a -> m b) -> m a -> m b
(>>=) :: Monad m => m a -> (a -> m b) -> m b
```

cf. (=<<) is just `(Control.Monad.join .) . fmap`
And (>>=) is just `(Control.Monad.join .) . flip fmap`


Defining the two in terms of each other.

```haskell
traverse :: (Traversable t, Applicative f) => (a -> f b) -> t a -> f (t b)
traverse f = sequenceA . fmap f 

sequenceA :: (Traversable t, Applicative f) => t (f a) -> f (t a)
sequenceA = traverse id 
```

n.b. With sequenceA, we turn the structure inside out, and because `t` is a Traversable and Traversables are Foldables, we return `f (t a)` with the `t a` folded.

Interesting syntax

```haskell
(sequence .) . fmap = \f xs -> sequence (fmap f xs)
sequence . fmap f = \xs -> (sequence . fmap) xs
sequence (fmap f xs)
```

### Laws for `traverse`

Naturality

```haskell
g . traverse f = traverse (g . f)
```

Identity

```haskell
traverse Identity = Identity
```

Composition

```haskell
traverse (Compose . fmap g . f) = Compose . fmap (traverse g) . traverse f
```

See IdentityTraversable.hs for a detailed example.

### Laws for `sequenceA`

Naturality

`t . sequenceA = sequenceA . fmap t` for every applicative t

Identity

```haskell
sequenceA . fmap Identiy = Identity
```

Composition

```haskell
sequenceA . fmap Compose = Compose . fmap sequenceA . sequenceA
```



How does this work?

```haskell
(fmap . fmap) sum Just [1, 2, 3]
```

Also, this

```haskell
sequenceA [[1, 2], [3, 4]]
-- [[1, 3], [1, 4], [2, 3], [2, 4]]
```

sequenceA [(+3), (+2), (+1)] 3
(+3) : ((+2) : ((+1) : []))

sequenceA [(+3), (+2), (+1)] :: Num a => (-> a [a])
returns an unary function that returns a list

We traverse through the list of functions [(+3), (+2), (+1)] and apply each function in turn before prepending the result to our list.

Consider: sequenceA [(+1)]
\x -> [x + 1]

And so: sequenceA [(+1), (+2)]
is simply
\x -> [x + 1, x + 2]
which is just syntactic sugar for
\x -> x + 1 : (x + 2 : []) :: Num a => a -> [a] 

So with the sequenceA function, we traverse a Traversable applying its elements in turn, hence the name 'sequence Applicative'