# Reader typeclass

It lets us put together functions awaiting input from a shared environment. We can abstract over functions that haven't been fully applied and send the same value to all of them.

A wrapper for the function type (->)

```haskell
newtype Reader r a =
  Reader { runReader :: r -> a }
```

cf. 'state' and 'props' in ReactJS and the problem of 'prop drilling'

```haskell
(+) <$> (*2) <*> (+10)
(+) (*2) <*> (+10)

<*> :: Applicative f => f (a -> b) -> f a -> f b 

-- f is ((->) a)
-- Substituting f gives us the following:
<*> :: ((->) a (a -> b)) -> ((->) a a) -> ((->) a b)
<*> :: (a -> (a -> b)) -> (a -> a) -> (a -> b)

-- The first argument to (<*>) denoted by 'a' is a function, namely, (a -> a). In this case, this will be the (+10) function.
-- Whereas the first argument to the second argument, also denoted by 'a', is an Integer. In this case, this will be the argument to (*2) and (+10).
```

The applicative context lets us apply a function to two functions awaiting application to a shared input.

### Functor typeclass instance for functions

The Functor for functions is just function composition

```haskell
fmap :: Functor f => (a -> b) -> f a -> f b

-- Suppose f is a function, namely '(->) r', then we have

fmap :: (a -> b) -> (->) r a -> (->) r b 

-- which is just

fmap :: (a -> b) -> (r -> a) -> (r -> b)

-- cf. (.)
(.) :: (b -> c) -> (a -> b) -> a -> c
```

n.b. the first argument to `(->) r a` is the argument type and the second argument is the return type


### Applicative typeclass instance for functions

```haskell
pure :: a -> f a
pure :: a -> (-> r) a 
pure :: a -> (r -> a)

-- cf. this is very similar to the conditional introduction inference rule in logic

(<*>) :: f (a -> b) -> f a -> f b 
(<*>) :: (->) r (a -> b) -> (->) r a -> (->) r b 
(<*>) :: (r -> a -> b) -> (r -> a) -> (r -> b)

-- Think of this as just <*> with an extra argument
-- Try visualising this using Gentzen-style natural deduction proof tree.
```

### Monad typeclass instance for functions

```haskell
'return' is basically the Monad version of 'pure'
return :: Monad m => a -> m a 
return :: a -> (-> r) a 
return :: a -> (r -> a)

>>= :: Applicative m => m a -> (a -> m b) -> m b

-- Type signature of (>>=) for functions
>>= :: (->) r a -> (a -> (->) r b) -> (->) r b 
>>= :: (r -> a) -> (a -> r -> b) -> r -> b

-- cf. Contrast this with the (<*>) defined for function types
<*> :: (r -> a -> b ) -> (r -> a) -> r -> b

-- Also compare with 'fmap'
<$> :: (a -> b) -> (r -> a) -> (r -> b)
```
